Make ITree.bind a function instead of a notation
Simplify some proofs

theories/Eq/Shallow.v
@@ -19,6 +19,8 @@ From Coq Require Import
      Setoids.Setoid
      Relations.Relations
      JMeq.
+
+Set Implicit Arguments.
 (* end hide *)
 
 Definition eqeq {A : Type} (P : A -> Type) {a1 a2 : A} (p : a1 = a2) : P a1 -> P a2 -> Prop :=
@@ -62,11 +64,11 @@ Ltac inv_Vis :=
   end.
 
 (** ** [observing]: Lift relations through [observe]. *)
-Inductive observing {E R1 R2}
+Record observing {E R1 R2}
            (eq_ : itree' E R1 -> itree' E R2 -> Prop)
            (t1 : itree E R1) (t2 : itree E R2) : Prop :=
-| observing_intros :
-    eq_ (observe t1) (observe t2) -> observing eq_ t1 t2.
+  observing_intros
+  { observing_observe : eq_ (observe t1) (observe t2) }.
 Hint Constructors observing: core.
 
 Section observing_relations.
@@ -74,7 +76,7 @@ Section observing_relations.
 Context {E : Type -> Type} {R : Type}.
 Variable (eq_ : itree' E R -> itree' E R -> Prop).
 
-Global Instance observing_observe :
+Global Instance observing_observe_ :
   Proper (observing eq_ ==> eq_) (@observe E R).
 Proof. intros ? ? []; cbv; auto. Qed.
 
@@ -98,34 +100,26 @@ End observing_relations.
 
 (** ** Unfolding lemmas for [bind] *)
 
-Lemma unfold_bind_ {E R S}
-      (t : itree E R) (k : R -> itree E S) :
-  observing eq
-    (ITree.bind t k)
-    (ITree._bind k (fun t => ITree.bind t k) (observe t)).
-Proof. eauto. Qed.
-
 Instance observing_bind {E R S} :
-  Proper (eq ==> observing eq ==> observing eq) (@ITree.bind' E R S).
+  Proper (observing eq ==> eq ==> observing eq) (@ITree.bind E R S).
 Proof.
-  repeat intro; subst.
-  do 2 rewrite unfold_bind_; rewrite H0.
-  reflexivity.
+  repeat intro; subst. constructor. unfold observe. cbn.
+  rewrite (observing_observe H). reflexivity.
 Qed.
 
 Lemma bind_ret_ {E R S} (r : R) (k : R -> itree E S) :
   observing eq (ITree.bind (Ret r) k) (k r).
-Proof. apply unfold_bind_. Qed.
+Proof. constructor; reflexivity. Qed.
 
 Lemma bind_tau_ {E R} U t (k: U -> itree E R) :
   observing eq (ITree.bind (Tau t) k) (Tau (ITree.bind t k)).
-Proof. apply @unfold_bind_. Qed.
+Proof. constructor; reflexivity. Qed.
 
 Lemma bind_vis_ {E R U V} (e: E V) (ek: V -> itree E U) (k: U -> itree E R) :
   observing eq
     (ITree.bind (Vis e ek) k)
     (Vis e (fun x => ITree.bind (ek x) k)).
-Proof. apply @unfold_bind_. Qed.
+Proof. constructor; reflexivity. Qed.
 
 (** Unfolding lemma for [aloop]. There is also a variant [unfold_aloop]
     without [Tau]. *)
@@ -133,9 +127,7 @@ Lemma unfold_aloop_ {E A B} (f : A -> itree E (A + B)) (x : A) :
   observing eq
     (ITree.iter f x)
     (ITree.bind (f x) (fun lr => ITree.on_left lr l (Tau (ITree.iter f l)))).
-Proof.
-  constructor; reflexivity.
-Qed.
+Proof. constructor; reflexivity. Qed.
 
 (** Unfolding lemma for [forever]. *)
 Lemma unfold_forever_ {E R S} (t: itree E R):
@@ -147,7 +139,7 @@ Proof. econstructor. reflexivity. Qed.
 Inductive going {E R1 R2} (r : itree E R1 -> itree E R2 -> Prop)
           (ot1 : itree' E R1) (ot2 : itree' E R2) : Prop :=
 | going_intros : r (go ot1) (go ot2) -> going r ot1 ot2.
-Hint Constructors going: core.
+Global Hint Constructors going: core.
 
 Lemma observing_going {E R1 R2} (eq_ : itree' E R1 -> itree' E R2 -> Prop) ot1 ot2 :
   going (observing eq_) ot1 ot2 <-> eq_ ot1 ot2.
