theories/Interp/RecursionFacts.v
@@ -93,12 +93,13 @@ Theorem interp_mrec_bind {U T} (t : itree _ U) (k : U -> itree _ T) :
 Proof.
   revert t k; ginit. pcofix CIH; intros.
   rewrite (unfold_interp_mrec _ t).
-  rewrite (unfold_bind t). (* TODO: should be [unfold_bind] but it is much slower *)
+  rewrite (unfold_bind t).
+  unfold observe at 1. cbn.
   destruct (observe t); cbn;
     [| |destruct e];
     autorewrite with itree.
-  1: apply reflexivity.
-  all: rewrite unfold_interp_mrec.
+  1: rewrite <- itree_eta_; apply reflexivity.
+  all: rewrite unfold_interp_mrec; ITree.fold_subst.
   all: try (gstep; econstructor; eauto with paco).
   - rewrite <- bind_bind; eauto with paco.
   - intros. red. rewrite bind_tau. gstep; constructor; auto with paco.
@@ -154,22 +155,24 @@ Theorem unfold_interp_mrec_h {T} (t : itree _ T)
 Proof.
   rewrite <- tau_eutt.
   revert t. ginit; pcofix CIH. intros.
-  rewrite (itree_eta t); destruct (observe t);
-    try (rewrite 2 unfold_interp_mrec; cbn; gstep; repeat constructor; auto with paco; fail).
-  rewrite interp_vis.
-  rewrite (unfold_interp_mrec _ (Vis _ _)).
-  destruct e; cbn.
-  - rewrite 2 interp_mrec_bind.
-    gstep; constructor.
-    guclo eqit_clo_bind; econstructor; [reflexivity|].
-    intros ? _ []; rewrite unfold_interp_mrec; cbn; auto with paco.
-  - unfold inr_, Handler.Inr_sum1_Handler, Handler.Handler.inr_, Handler.Handler.htrigger.
-    rewrite bind_trigger, unfold_interp_mrec; cbn.
-    rewrite tau_euttge.
-    gstep; constructor.
-    intros; red. gstep; constructor.
-    rewrite unfold_interp_mrec; cbn.
-    auto with paco.
+  rewrite (itree_eta t); destruct (observe t).
+  - rewrite 2 unfold_interp_mrec; cbn; gstep; repeat constructor; auto with paco.
+  - rewrite unfold_interp, 2 unfold_interp_mrec; cbn. gstep.
+    constructor; auto with paco.
+  - rewrite interp_vis.
+    rewrite (unfold_interp_mrec _ (Vis _ _)).
+    destruct e; cbn.
+    + rewrite 2 interp_mrec_bind.
+      gstep; constructor.
+      guclo eqit_clo_bind; econstructor; [reflexivity|].
+      intros ? _ []; rewrite unfold_interp_mrec; cbn; auto with paco.
+    + unfold inr_, Handler.Inr_sum1_Handler, Handler.Handler.inr_, Handler.Handler.htrigger.
+      rewrite bind_trigger, unfold_interp_mrec; cbn.
+      rewrite tau_euttge.
+      gstep; constructor.
+      intros; red. gstep; constructor.
+      rewrite unfold_interp_mrec; cbn.
+      auto with paco.
 Qed.
 
 End Facts.
